LLVM_DS_RBT/Export.thy
@@ -1,7 +1,7 @@
 theory Export
   imports
     Delete
-    Balance
+    "Insert/Insert"
     Lookup
     "Insert/Naive_Insert"
 begin
@@ -21,6 +21,8 @@ global_interpretation unat_rbt: rbt_impl
   key_delete 
   defines 
     unat_rbt_naive_insert = unat_rbt.naive_insert and
+    unat_rbt_balance = unat_rbt.balance and
+    unat_rbt_insert = unat_rbt.insert and
     unat_rbt_empty = unat_rbt.empty and
     unat_rbt_lookup = unat_rbt.lookup
 proof(standard, goal_cases)
@@ -41,17 +43,20 @@ next
 qed
 
 
-lemmas [llvm_code] = unat_rbt.naive_insert.simps unat_rbt.empty_def unat_rbt.lookup.simps
-
-
 abbreviation unat_rbt_naive_insert_64 :: 
   "(64 word, 8 word) rbt_node ptr \<Rightarrow> _"        
   where "unat_rbt_naive_insert_64 \<equiv> unat_rbt_naive_insert"
 
+abbreviation unat_rbt_insert_64 :: 
+  "_ \<Rightarrow> _ \<Rightarrow> (64 word, 8 word) rbt_node ptr \<Rightarrow> _"        
+  where "unat_rbt_insert_64 \<equiv> unat_rbt_insert"
+
+abbreviation unat_rbt_balance_64 :: 
+  "(64 word, 8 word) rbt_node ptr \<Rightarrow> _"        
+  where "unat_rbt_balance_64 \<equiv> unat_rbt_balance"
 
 abbreviation unat_rbt_empty_64 :: "(64 word, 8 word) rbti llM"
   where "unat_rbt_empty_64 \<equiv> unat_rbt_empty"
-
 
 abbreviation unat_rbt_lookup_64 :: "(64 word, 8 word) rbti \<Rightarrow> _"
   where "unat_rbt_lookup_64 \<equiv> unat_rbt_lookup"
@@ -59,7 +64,9 @@ abbreviation unat_rbt_lookup_64 :: "(64 word, 8 word) rbti \<Rightarrow> _"
 
 export_llvm
   unat_rbt_empty_64 is "rbt_node* empty()"  
-  unat_rbt_naive_insert_64 is "rbt_node* insert(rbt_node*, uint64_t, uint8_t)"
+  unat_rbt_naive_insert_64 is "rbt_node* naive_insert(rbt_node*, uint64_t, uint8_t)"
+  unat_rbt_insert_64 is "rbt_node* insert(uint64_t, uint8_t, rbt_node*)"
+  unat_rbt_balance_64 is "rbt_node* balance(rbt_node*, uint64_t, uint8_t, rbt_node*)"
   unat_rbt_lookup_64 is "option_i* lookup(rbt_node*, uint64_t)"
   defines \<open>
     typedef struct {
