LLVM_DS_RBT/Insert/Insert.thy
@@ -1,0 +1,227 @@
+theory Insert
+  imports Balance
+begin
+
+
+fun rbt_insert_ad' where
+  "rbt_insert_ad' k\<^sub>n v\<^sub>n rbt.Empty = Branch color.R rbt.Empty k\<^sub>n v\<^sub>n rbt.Empty"
+| "rbt_insert_ad' k\<^sub>n v\<^sub>n (Branch color.B l k v r) = (
+    if k\<^sub>n < k then rbt_balance (rbt_insert_ad' k\<^sub>n v\<^sub>n l) k v r
+    else if k\<^sub>n > k then rbt_balance l k v (rbt_insert_ad' k\<^sub>n v\<^sub>n r)
+    else Branch color.B l k\<^sub>n v\<^sub>n r
+  )"
+| "rbt_insert_ad' k\<^sub>n v\<^sub>n (Branch color.R l k v r) = (
+    if k\<^sub>n < k then Branch color.R (rbt_insert_ad' k\<^sub>n v\<^sub>n l) k v r
+    else if k\<^sub>n > k then Branch color.R l k v (rbt_insert_ad' k\<^sub>n v\<^sub>n r)
+    else Branch color.R l k\<^sub>n v\<^sub>n r
+  )"
+
+
+definition rbt_insert_ad where
+  "rbt_insert_ad k v t = paint color.B (rbt_insert_ad' k v t)"
+
+
+lemma rbt_insert_ad'_correct: 
+  "rbt_insert_ad' k v t = rbt_ins (\<lambda>_ _ nv. nv) k v t"
+  by (induction k v t rule: rbt_insert_ad'.induct; auto)
+  
+  
+lemma rbt_insert_ad_correct:
+  "rbt_insert_ad k v t = rbt_insert k v t"
+  unfolding rbt_insert_def rbt_insert_ad_def rbt_insert_with_key_def
+  using rbt_insert_ad'_correct 
+  by (rule arg_cong)
+
+
+context rbt_impl
+begin 
+
+
+definition X :: "'a \<Rightarrow> 'a llM" where  "X x = Mreturn x"
+
+partial_function (M) insertt where
+  "insertt x = do {
+    z \<leftarrow> insertt x;
+    a \<leftarrow> X z;
+    return a
+  }"
+
+
+partial_function (M) insert' ::
+  "'ki \<Rightarrow> 'v::llvm_rep \<Rightarrow> ('ki, 'v) rbti \<Rightarrow> ('ki, 'v) rbti llM" where
+  "insert' k\<^sub>n v\<^sub>n n_p = do {
+    if n_p = null
+    then new (RBT_NODE 0 null k\<^sub>n v\<^sub>n null)
+    else do {
+      n \<leftarrow> ll_load n_p;
+      ll_free n_p;
+      case n of (RBT_NODE col l k v r) \<Rightarrow>      
+      do {
+        if col = 0
+        then do {
+          c1 \<leftarrow> lt_impl k\<^sub>n k;
+          if c1 = 1
+          then  do { l\<^sub>n \<leftarrow> insert' k\<^sub>n v\<^sub>n l; new (RBT_NODE 0 l\<^sub>n k v r) }
+          else do {
+            c2 \<leftarrow> lt_impl k k\<^sub>n;
+            if c2 = 1
+            then do { r\<^sub>n \<leftarrow> insert' k\<^sub>n v\<^sub>n r; new (RBT_NODE 0 l k v r\<^sub>n) }
+            else do {
+              key_delete k;
+              new (RBT_NODE 0 l k\<^sub>n v\<^sub>n r)
+            }
+          }
+        }
+        else do {
+          c1 \<leftarrow> lt_impl k\<^sub>n k;
+          if c1 = 1
+          then do { l\<^sub>n \<leftarrow> insert' k\<^sub>n v\<^sub>n l; balance l\<^sub>n k v r }
+          else do {
+            c2 \<leftarrow> lt_impl k k\<^sub>n;
+            if c2 = 1
+            then do { r\<^sub>n \<leftarrow> insert' k\<^sub>n v\<^sub>n r; balance l k v r\<^sub>n }
+            else do {
+              key_delete k;
+              new (RBT_NODE 1 l k\<^sub>n v\<^sub>n r)
+            }
+          }
+        }
+      }
+    }
+  }"
+
+
+lemma insert'_correct:
+  "
+    llvm_htriple
+    (\<upharpoonleft>rbt_assn tree treei ** \<upharpoonleft>key_assn k ki)
+    (insert' ki v treei)
+    (\<lambda>r. \<upharpoonleft>rbt_assn (rbt_insert_ad' k v tree) r)
+  "
+proof (induction k v tree arbitrary: treei ki v rule: rbt_insert_ad'.induct)
+  case (1 k\<^sub>n v\<^sub>n)
+  then show ?case
+    apply (subst insert'.simps)
+    apply vcg
+    unfolding rbt_assn_branch_def
+    apply vcg
+    done
+next
+  case (2 k\<^sub>n v\<^sub>n l k v r)
+  
+  note [vcg_rules] = 2
+
+  have color_contr_B: "\<not>\<flat>\<^sub>pcolor_assn B 0"
+    by (simp add: color_assn_def dr_assn_prefix_def dr_assn_pure_asm_prefix_def mk_assn_def)
+
+  from color_contr_B show ?case
+    apply (subst insert'.simps)
+    apply vcg
+    apply simp
+    unfolding rbt_assn_branch_def 
+    apply vcg
+    done
+next
+  case (3 k\<^sub>n v\<^sub>n l k v r)
+
+  note [vcg_rules] = 3
+
+  have color_contr_R: "\<flat>\<^sub>pcolor_assn R x \<Longrightarrow> x = 0" for x
+    by (simp add: color_assn_def dr_assn_prefix_def dr_assn_pure_asm_prefix_def mk_assn_def)
+
+  from color_contr_R show ?case
+    apply (subst insert'.simps)
+    apply vcg
+    subgoal (*case left*)
+      apply simp
+      unfolding rbt_assn_branch_def
+      apply vcg
+      done
+    subgoal (*cases right, equal*)
+      apply vcg
+      subgoal (*case right*)
+        apply simp
+        unfolding rbt_assn_branch_def
+        apply vcg
+        done
+      subgoal (*case equal*)
+        apply vcg
+        apply simp
+        unfolding rbt_assn_branch_def
+        apply vcg
+        done
+      done
+    done
+qed
+
+
+lemmas [llvm_code] = insert'.simps
+
+
+definition insert where "insert k v tree \<equiv> do {
+  r_p \<leftarrow> insert' k v tree;
+  r \<leftarrow> ll_load r_p;
+  r_colored \<leftarrow> (set_color r 1);
+  ll_store r_colored r_p;
+  return r_p
+}"
+
+lemma rbt_balance_unfold:
+  obtains c l' k' v' r' where "rbt_balance l k v r = Branch c l' k' v' r'"
+  apply(cases "(l, k, v ,r)" rule: RBT_Impl.balance.cases)
+  by auto
+
+lemma rbt_balance_non_empty:
+  "rbt_balance l k v r \<noteq> rbt.Empty"
+  by (metis rbt_balance_unfold rbt.simps(3))
+  
+
+lemma rbt_insert_ad'_non_empty:
+  "rbt_insert_ad' k v tree \<noteq> rbt.Empty"
+  apply(cases "(k, v, tree)" rule: rbt_insert_ad'.cases)
+  by (simp add: rbt_balance_non_empty)+
+
+
+lemma *: "\<upharpoonleft>\<^sub>pcolor_assn B 1 = \<up>True"
+  by (simp add: dr_assn_pure_prefix_def)
+
+
+lemma insert_correct':
+  "
+    llvm_htriple
+    (\<upharpoonleft>rbt_assn tree treei ** \<upharpoonleft>key_assn k ki)
+    (insert ki v treei)
+    (\<lambda>r. \<upharpoonleft>rbt_assn (rbt_insert_ad k v tree) r)
+  "
+  unfolding insert_def rbt_insert_ad_def
+  supply insert'_correct [vcg_rules]
+  apply vcg
+  apply (cases "rbt_insert_ad' k v tree")
+  subgoal using rbt_insert_ad'_non_empty by fast
+  subgoal
+    apply simp
+    unfolding rbt_assn_branch_def
+    apply vcg
+    supply *[simp]
+    apply vcg_try_solve
+    by (simp add: bury_pure_assn' fri_end)
+  done
+
+
+lemma insert_correct [vcg_rules]:
+  "
+    llvm_htriple
+    (\<upharpoonleft>rbt_assn tree treei ** \<upharpoonleft>key_assn k ki)
+    (insert ki v treei)
+    (\<lambda>r. \<upharpoonleft>rbt_assn (rbt_insert k v tree) r)
+  " 
+  using insert_correct' rbt_insert_ad_correct by metis
+
+
+lemmas [llvm_code] = insert_def
+
+
+end
+
+
+end
