LLVM_DS_RBT/OptionI.thy
@@ -1,5 +1,5 @@
 theory OptionI
-  imports "Isabelle_LLVM.LLVM_DS_All"
+  imports Isabelle_LLVM.LLVM_DS_Dflt
   Main
 begin
 
